# The preunivalence axiom

<pre class="Agda"><a id="36" class="Keyword">module</a> <a id="43" href="foundation.preunivalence.html" class="Module">foundation.preunivalence</a> <a id="68" class="Keyword">where</a>
</pre>
<details><summary>Imports</summary>

<pre class="Agda"><a id="124" class="Keyword">open</a> <a id="129" class="Keyword">import</a> <a id="136" href="foundation.dependent-pair-types.html" class="Module">foundation.dependent-pair-types</a>
<a id="168" class="Keyword">open</a> <a id="173" class="Keyword">import</a> <a id="180" href="foundation.embeddings.html" class="Module">foundation.embeddings</a>
<a id="202" class="Keyword">open</a> <a id="207" class="Keyword">import</a> <a id="214" href="foundation.equivalences.html" class="Module">foundation.equivalences</a>
<a id="238" class="Keyword">open</a> <a id="243" class="Keyword">import</a> <a id="250" href="foundation.sets.html" class="Module">foundation.sets</a>
<a id="266" class="Keyword">open</a> <a id="271" class="Keyword">import</a> <a id="278" href="foundation.univalence.html" class="Module">foundation.univalence</a>
<a id="300" class="Keyword">open</a> <a id="305" class="Keyword">import</a> <a id="312" href="foundation.universe-levels.html" class="Module">foundation.universe-levels</a>

<a id="340" class="Keyword">open</a> <a id="345" class="Keyword">import</a> <a id="352" href="foundation-core.identity-types.html" class="Module">foundation-core.identity-types</a>
<a id="383" class="Keyword">open</a> <a id="388" class="Keyword">import</a> <a id="395" href="foundation-core.subtypes.html" class="Module">foundation-core.subtypes</a>
</pre>
</details>

## Idea

**The preunivalence axiom**, or **axiom L**, which is due to Peter Lumsdaine,
asserts that for any two types `X` and `Y` in a common universe, the map
`X ＝ Y → X ≃ Y` is an [embedding](foundation-core.embeddings.md). This axiom is
a common generalization of the [univalence axiom](foundation.univalence.md) and
[axiom K](foundation-core.sets.md).

## Definition

<pre class="Agda"><a id="instance-preunivalence"></a><a id="817" href="foundation.preunivalence.html#817" class="Function">instance-preunivalence</a> <a id="840" class="Symbol">:</a> <a id="842" class="Symbol">{</a><a id="843" href="foundation.preunivalence.html#843" class="Bound">l</a> <a id="845" class="Symbol">:</a> <a id="847" href="Agda.Primitive.html#742" class="Postulate">Level</a><a id="852" class="Symbol">}</a> <a id="854" class="Symbol">(</a><a id="855" href="foundation.preunivalence.html#855" class="Bound">X</a> <a id="857" href="foundation.preunivalence.html#857" class="Bound">Y</a> <a id="859" class="Symbol">:</a> <a id="861" href="Agda.Primitive.html#388" class="Primitive">UU</a> <a id="864" href="foundation.preunivalence.html#843" class="Bound">l</a><a id="865" class="Symbol">)</a> <a id="867" class="Symbol">→</a> <a id="869" href="Agda.Primitive.html#388" class="Primitive">UU</a> <a id="872" class="Symbol">(</a><a id="873" href="Agda.Primitive.html#931" class="Primitive">lsuc</a> <a id="878" href="foundation.preunivalence.html#843" class="Bound">l</a><a id="879" class="Symbol">)</a>
<a id="881" href="foundation.preunivalence.html#817" class="Function">instance-preunivalence</a> <a id="904" href="foundation.preunivalence.html#904" class="Bound">X</a> <a id="906" href="foundation.preunivalence.html#906" class="Bound">Y</a> <a id="908" class="Symbol">=</a> <a id="910" href="foundation-core.embeddings.html#1086" class="Function">is-emb</a> <a id="917" class="Symbol">(</a><a id="918" href="foundation-core.univalence.html#855" class="Function">equiv-eq</a> <a id="927" class="Symbol">{</a><a id="928" class="Argument">A</a> <a id="930" class="Symbol">=</a> <a id="932" href="foundation.preunivalence.html#904" class="Bound">X</a><a id="933" class="Symbol">}</a> <a id="935" class="Symbol">{</a><a id="936" class="Argument">B</a> <a id="938" class="Symbol">=</a> <a id="940" href="foundation.preunivalence.html#906" class="Bound">Y</a><a id="941" class="Symbol">})</a>

<a id="based-preunivalence-axiom"></a><a id="945" href="foundation.preunivalence.html#945" class="Function">based-preunivalence-axiom</a> <a id="971" class="Symbol">:</a> <a id="973" class="Symbol">{</a><a id="974" href="foundation.preunivalence.html#974" class="Bound">l</a> <a id="976" class="Symbol">:</a> <a id="978" href="Agda.Primitive.html#742" class="Postulate">Level</a><a id="983" class="Symbol">}</a> <a id="985" class="Symbol">(</a><a id="986" href="foundation.preunivalence.html#986" class="Bound">X</a> <a id="988" class="Symbol">:</a> <a id="990" href="Agda.Primitive.html#388" class="Primitive">UU</a> <a id="993" href="foundation.preunivalence.html#974" class="Bound">l</a><a id="994" class="Symbol">)</a> <a id="996" class="Symbol">→</a> <a id="998" href="Agda.Primitive.html#388" class="Primitive">UU</a> <a id="1001" class="Symbol">(</a><a id="1002" href="Agda.Primitive.html#931" class="Primitive">lsuc</a> <a id="1007" href="foundation.preunivalence.html#974" class="Bound">l</a><a id="1008" class="Symbol">)</a>
<a id="1010" href="foundation.preunivalence.html#945" class="Function">based-preunivalence-axiom</a> <a id="1036" class="Symbol">{</a><a id="1037" href="foundation.preunivalence.html#1037" class="Bound">l</a><a id="1038" class="Symbol">}</a> <a id="1040" href="foundation.preunivalence.html#1040" class="Bound">X</a> <a id="1042" class="Symbol">=</a> <a id="1044" class="Symbol">(</a><a id="1045" href="foundation.preunivalence.html#1045" class="Bound">Y</a> <a id="1047" class="Symbol">:</a> <a id="1049" href="Agda.Primitive.html#388" class="Primitive">UU</a> <a id="1052" href="foundation.preunivalence.html#1037" class="Bound">l</a><a id="1053" class="Symbol">)</a> <a id="1055" class="Symbol">→</a> <a id="1057" href="foundation.preunivalence.html#817" class="Function">instance-preunivalence</a> <a id="1080" href="foundation.preunivalence.html#1040" class="Bound">X</a> <a id="1082" href="foundation.preunivalence.html#1045" class="Bound">Y</a>

<a id="preunivalence-axiom-Level"></a><a id="1085" href="foundation.preunivalence.html#1085" class="Function">preunivalence-axiom-Level</a> <a id="1111" class="Symbol">:</a> <a id="1113" class="Symbol">(</a><a id="1114" href="foundation.preunivalence.html#1114" class="Bound">l</a> <a id="1116" class="Symbol">:</a> <a id="1118" href="Agda.Primitive.html#742" class="Postulate">Level</a><a id="1123" class="Symbol">)</a> <a id="1125" class="Symbol">→</a> <a id="1127" href="Agda.Primitive.html#388" class="Primitive">UU</a> <a id="1130" class="Symbol">(</a><a id="1131" href="Agda.Primitive.html#931" class="Primitive">lsuc</a> <a id="1136" href="foundation.preunivalence.html#1114" class="Bound">l</a><a id="1137" class="Symbol">)</a>
<a id="1139" href="foundation.preunivalence.html#1085" class="Function">preunivalence-axiom-Level</a> <a id="1165" href="foundation.preunivalence.html#1165" class="Bound">l</a> <a id="1167" class="Symbol">=</a> <a id="1169" class="Symbol">(</a><a id="1170" href="foundation.preunivalence.html#1170" class="Bound">X</a> <a id="1172" href="foundation.preunivalence.html#1172" class="Bound">Y</a> <a id="1174" class="Symbol">:</a> <a id="1176" href="Agda.Primitive.html#388" class="Primitive">UU</a> <a id="1179" href="foundation.preunivalence.html#1165" class="Bound">l</a><a id="1180" class="Symbol">)</a> <a id="1182" class="Symbol">→</a> <a id="1184" href="foundation.preunivalence.html#817" class="Function">instance-preunivalence</a> <a id="1207" href="foundation.preunivalence.html#1170" class="Bound">X</a> <a id="1209" href="foundation.preunivalence.html#1172" class="Bound">Y</a>

<a id="preunivalence-axiom"></a><a id="1212" href="foundation.preunivalence.html#1212" class="Function">preunivalence-axiom</a> <a id="1232" class="Symbol">:</a> <a id="1234" href="Agda.Primitive.html#512" class="Primitive">UUω</a>
<a id="1238" href="foundation.preunivalence.html#1212" class="Function">preunivalence-axiom</a> <a id="1258" class="Symbol">=</a> <a id="1260" class="Symbol">{</a><a id="1261" href="foundation.preunivalence.html#1261" class="Bound">l</a> <a id="1263" class="Symbol">:</a> <a id="1265" href="Agda.Primitive.html#742" class="Postulate">Level</a><a id="1270" class="Symbol">}</a> <a id="1272" class="Symbol">→</a> <a id="1274" href="foundation.preunivalence.html#1085" class="Function">preunivalence-axiom-Level</a> <a id="1300" href="foundation.preunivalence.html#1261" class="Bound">l</a>

<a id="emb-preunivalence"></a><a id="1303" href="foundation.preunivalence.html#1303" class="Function">emb-preunivalence</a> <a id="1321" class="Symbol">:</a>
  <a id="1325" href="foundation.preunivalence.html#1212" class="Function">preunivalence-axiom</a> <a id="1345" class="Symbol">→</a> <a id="1347" class="Symbol">{</a><a id="1348" href="foundation.preunivalence.html#1348" class="Bound">l</a> <a id="1350" class="Symbol">:</a> <a id="1352" href="Agda.Primitive.html#742" class="Postulate">Level</a><a id="1357" class="Symbol">}</a> <a id="1359" class="Symbol">(</a><a id="1360" href="foundation.preunivalence.html#1360" class="Bound">X</a> <a id="1362" href="foundation.preunivalence.html#1362" class="Bound">Y</a> <a id="1364" class="Symbol">:</a> <a id="1366" href="Agda.Primitive.html#388" class="Primitive">UU</a> <a id="1369" href="foundation.preunivalence.html#1348" class="Bound">l</a><a id="1370" class="Symbol">)</a> <a id="1372" class="Symbol">→</a> <a id="1374" class="Symbol">(</a><a id="1375" href="foundation.preunivalence.html#1360" class="Bound">X</a> <a id="1377" href="foundation-core.identity-types.html#1953" class="Function Operator">＝</a> <a id="1379" href="foundation.preunivalence.html#1362" class="Bound">Y</a><a id="1380" class="Symbol">)</a> <a id="1382" href="foundation-core.embeddings.html#1495" class="Function Operator">↪</a> <a id="1384" class="Symbol">(</a><a id="1385" href="foundation.preunivalence.html#1360" class="Bound">X</a> <a id="1387" href="foundation-core.equivalences.html#2669" class="Function Operator">≃</a> <a id="1389" href="foundation.preunivalence.html#1362" class="Bound">Y</a><a id="1390" class="Symbol">)</a>
<a id="1392" href="foundation.dependent-pair-types.html#603" class="Field">pr1</a> <a id="1396" class="Symbol">(</a><a id="1397" href="foundation.preunivalence.html#1303" class="Function">emb-preunivalence</a> <a id="1415" href="foundation.preunivalence.html#1415" class="Bound">L</a> <a id="1417" href="foundation.preunivalence.html#1417" class="Bound">X</a> <a id="1419" href="foundation.preunivalence.html#1419" class="Bound">Y</a><a id="1420" class="Symbol">)</a> <a id="1422" class="Symbol">=</a> <a id="1424" href="foundation-core.univalence.html#855" class="Function">equiv-eq</a>
<a id="1433" href="foundation.dependent-pair-types.html#615" class="Field">pr2</a> <a id="1437" class="Symbol">(</a><a id="1438" href="foundation.preunivalence.html#1303" class="Function">emb-preunivalence</a> <a id="1456" href="foundation.preunivalence.html#1456" class="Bound">L</a> <a id="1458" href="foundation.preunivalence.html#1458" class="Bound">X</a> <a id="1460" href="foundation.preunivalence.html#1460" class="Bound">Y</a><a id="1461" class="Symbol">)</a> <a id="1463" class="Symbol">=</a> <a id="1465" href="foundation.preunivalence.html#1456" class="Bound">L</a> <a id="1467" href="foundation.preunivalence.html#1458" class="Bound">X</a> <a id="1469" href="foundation.preunivalence.html#1460" class="Bound">Y</a>

<a id="emb-map-preunivalence"></a><a id="1472" href="foundation.preunivalence.html#1472" class="Function">emb-map-preunivalence</a> <a id="1494" class="Symbol">:</a>
  <a id="1498" href="foundation.preunivalence.html#1212" class="Function">preunivalence-axiom</a> <a id="1518" class="Symbol">→</a> <a id="1520" class="Symbol">{</a><a id="1521" href="foundation.preunivalence.html#1521" class="Bound">l</a> <a id="1523" class="Symbol">:</a> <a id="1525" href="Agda.Primitive.html#742" class="Postulate">Level</a><a id="1530" class="Symbol">}</a> <a id="1532" class="Symbol">(</a><a id="1533" href="foundation.preunivalence.html#1533" class="Bound">X</a> <a id="1535" href="foundation.preunivalence.html#1535" class="Bound">Y</a> <a id="1537" class="Symbol">:</a> <a id="1539" href="Agda.Primitive.html#388" class="Primitive">UU</a> <a id="1542" href="foundation.preunivalence.html#1521" class="Bound">l</a><a id="1543" class="Symbol">)</a> <a id="1545" class="Symbol">→</a> <a id="1547" class="Symbol">(</a><a id="1548" href="foundation.preunivalence.html#1533" class="Bound">X</a> <a id="1550" href="foundation-core.identity-types.html#1953" class="Function Operator">＝</a> <a id="1552" href="foundation.preunivalence.html#1535" class="Bound">Y</a><a id="1553" class="Symbol">)</a> <a id="1555" href="foundation-core.embeddings.html#1495" class="Function Operator">↪</a> <a id="1557" class="Symbol">(</a><a id="1558" href="foundation.preunivalence.html#1533" class="Bound">X</a> <a id="1560" class="Symbol">→</a> <a id="1562" href="foundation.preunivalence.html#1535" class="Bound">Y</a><a id="1563" class="Symbol">)</a>
<a id="1565" href="foundation.preunivalence.html#1472" class="Function">emb-map-preunivalence</a> <a id="1587" href="foundation.preunivalence.html#1587" class="Bound">L</a> <a id="1589" href="foundation.preunivalence.html#1589" class="Bound">X</a> <a id="1591" href="foundation.preunivalence.html#1591" class="Bound">Y</a> <a id="1593" class="Symbol">=</a>
  <a id="1597" href="foundation.embeddings.html#3582" class="Function">comp-emb</a> <a id="1606" class="Symbol">(</a><a id="1607" href="foundation-core.subtypes.html#4988" class="Function">emb-subtype</a> <a id="1619" href="foundation.equivalences.html#11279" class="Function">is-equiv-Prop</a><a id="1632" class="Symbol">)</a> <a id="1634" class="Symbol">(</a><a id="1635" href="foundation.preunivalence.html#1303" class="Function">emb-preunivalence</a> <a id="1653" href="foundation.preunivalence.html#1587" class="Bound">L</a> <a id="1655" href="foundation.preunivalence.html#1589" class="Bound">X</a> <a id="1657" href="foundation.preunivalence.html#1591" class="Bound">Y</a><a id="1658" class="Symbol">)</a>
</pre>
## Properties

### Preunivalence generalizes axiom K

To show that preunivalence generalizes axiom K, we assume axiom K for the types
in question and for the universe itself.

<pre class="Agda"><a id="1849" class="Keyword">module</a> <a id="1856" href="foundation.preunivalence.html#1856" class="Module">_</a>
  <a id="1860" class="Symbol">{</a><a id="1861" href="foundation.preunivalence.html#1861" class="Bound">l</a> <a id="1863" class="Symbol">:</a> <a id="1865" href="Agda.Primitive.html#742" class="Postulate">Level</a><a id="1870" class="Symbol">}</a> <a id="1872" class="Symbol">(</a><a id="1873" href="foundation.preunivalence.html#1873" class="Bound">A</a> <a id="1875" href="foundation.preunivalence.html#1875" class="Bound">B</a> <a id="1877" class="Symbol">:</a> <a id="1879" href="Agda.Primitive.html#388" class="Primitive">UU</a> <a id="1882" href="foundation.preunivalence.html#1861" class="Bound">l</a><a id="1883" class="Symbol">)</a>
  <a id="1887" class="Keyword">where</a>

  <a id="1896" href="foundation.preunivalence.html#1896" class="Function">instance-preunivalence-instance-axiom-K</a> <a id="1936" class="Symbol">:</a>
    <a id="1942" href="foundation-core.sets.html#1113" class="Function">instance-axiom-K</a> <a id="1959" class="Symbol">(</a><a id="1960" href="Agda.Primitive.html#388" class="Primitive">UU</a> <a id="1963" href="foundation.preunivalence.html#1861" class="Bound">l</a><a id="1964" class="Symbol">)</a> <a id="1966" class="Symbol">→</a> <a id="1968" href="foundation-core.sets.html#1113" class="Function">instance-axiom-K</a> <a id="1985" href="foundation.preunivalence.html#1873" class="Bound">A</a> <a id="1987" class="Symbol">→</a> <a id="1989" href="foundation-core.sets.html#1113" class="Function">instance-axiom-K</a> <a id="2006" href="foundation.preunivalence.html#1875" class="Bound">B</a> <a id="2008" class="Symbol">→</a>
    <a id="2014" href="foundation.preunivalence.html#817" class="Function">instance-preunivalence</a> <a id="2037" href="foundation.preunivalence.html#1873" class="Bound">A</a> <a id="2039" href="foundation.preunivalence.html#1875" class="Bound">B</a>
  <a id="2043" href="foundation.preunivalence.html#1896" class="Function">instance-preunivalence-instance-axiom-K</a> <a id="2083" href="foundation.preunivalence.html#2083" class="Bound">K-Type</a> <a id="2090" href="foundation.preunivalence.html#2090" class="Bound">K-A</a> <a id="2094" href="foundation.preunivalence.html#2094" class="Bound">K-B</a> <a id="2098" class="Symbol">=</a>
    <a id="2104" href="foundation.sets.html#6275" class="Function">is-emb-is-prop-is-set</a>
      <a id="2132" class="Symbol">(</a> <a id="2134" href="foundation-core.sets.html#1584" class="Function">is-set-axiom-K</a> <a id="2149" href="foundation.preunivalence.html#2083" class="Bound">K-Type</a> <a id="2156" href="foundation.preunivalence.html#1873" class="Bound">A</a> <a id="2158" href="foundation.preunivalence.html#1875" class="Bound">B</a><a id="2159" class="Symbol">)</a>
      <a id="2167" class="Symbol">(</a> <a id="2169" href="foundation.sets.html#4578" class="Function">is-set-equiv-is-set</a> <a id="2189" class="Symbol">(</a><a id="2190" href="foundation-core.sets.html#1584" class="Function">is-set-axiom-K</a> <a id="2205" href="foundation.preunivalence.html#2090" class="Bound">K-A</a><a id="2208" class="Symbol">)</a> <a id="2210" class="Symbol">(</a><a id="2211" href="foundation-core.sets.html#1584" class="Function">is-set-axiom-K</a> <a id="2226" href="foundation.preunivalence.html#2094" class="Bound">K-B</a><a id="2229" class="Symbol">))</a>

<a id="preunivalence-axiom-axiom-K"></a><a id="2233" href="foundation.preunivalence.html#2233" class="Function">preunivalence-axiom-axiom-K</a> <a id="2261" class="Symbol">:</a> <a id="2263" href="foundation-core.sets.html#1304" class="Function">axiom-K</a> <a id="2271" class="Symbol">→</a> <a id="2273" href="foundation.preunivalence.html#1212" class="Function">preunivalence-axiom</a>
<a id="2293" href="foundation.preunivalence.html#2233" class="Function">preunivalence-axiom-axiom-K</a> <a id="2321" href="foundation.preunivalence.html#2321" class="Bound">K</a> <a id="2323" class="Symbol">{</a><a id="2324" href="foundation.preunivalence.html#2324" class="Bound">l</a><a id="2325" class="Symbol">}</a> <a id="2327" href="foundation.preunivalence.html#2327" class="Bound">X</a> <a id="2329" href="foundation.preunivalence.html#2329" class="Bound">Y</a> <a id="2331" class="Symbol">=</a>
  <a id="2335" href="foundation.preunivalence.html#1896" class="Function">instance-preunivalence-instance-axiom-K</a> <a id="2375" href="foundation.preunivalence.html#2327" class="Bound">X</a> <a id="2377" href="foundation.preunivalence.html#2329" class="Bound">Y</a> <a id="2379" class="Symbol">(</a><a id="2380" href="foundation.preunivalence.html#2321" class="Bound">K</a> <a id="2382" class="Symbol">(</a><a id="2383" href="Agda.Primitive.html#388" class="Primitive">UU</a> <a id="2386" href="foundation.preunivalence.html#2324" class="Bound">l</a><a id="2387" class="Symbol">))</a> <a id="2390" class="Symbol">(</a><a id="2391" href="foundation.preunivalence.html#2321" class="Bound">K</a> <a id="2393" href="foundation.preunivalence.html#2327" class="Bound">X</a><a id="2394" class="Symbol">)</a> <a id="2396" class="Symbol">(</a><a id="2397" href="foundation.preunivalence.html#2321" class="Bound">K</a> <a id="2399" href="foundation.preunivalence.html#2329" class="Bound">Y</a><a id="2400" class="Symbol">)</a>
</pre>
### Preunivalence generalizes univalence

<pre class="Agda"><a id="2457" class="Keyword">module</a> <a id="2464" href="foundation.preunivalence.html#2464" class="Module">_</a>
  <a id="2468" class="Symbol">{</a><a id="2469" href="foundation.preunivalence.html#2469" class="Bound">l</a> <a id="2471" class="Symbol">:</a> <a id="2473" href="Agda.Primitive.html#742" class="Postulate">Level</a><a id="2478" class="Symbol">}</a> <a id="2480" class="Symbol">(</a><a id="2481" href="foundation.preunivalence.html#2481" class="Bound">A</a> <a id="2483" href="foundation.preunivalence.html#2483" class="Bound">B</a> <a id="2485" class="Symbol">:</a> <a id="2487" href="Agda.Primitive.html#388" class="Primitive">UU</a> <a id="2490" href="foundation.preunivalence.html#2469" class="Bound">l</a><a id="2491" class="Symbol">)</a>
  <a id="2495" class="Keyword">where</a>

  <a id="2504" href="foundation.preunivalence.html#2504" class="Function">instance-preunivalence-instance-univalence</a> <a id="2547" class="Symbol">:</a>
    <a id="2553" href="foundation-core.univalence.html#1032" class="Function">instance-univalence</a> <a id="2573" href="foundation.preunivalence.html#2481" class="Bound">A</a> <a id="2575" href="foundation.preunivalence.html#2483" class="Bound">B</a> <a id="2577" class="Symbol">→</a> <a id="2579" href="foundation.preunivalence.html#817" class="Function">instance-preunivalence</a> <a id="2602" href="foundation.preunivalence.html#2481" class="Bound">A</a> <a id="2604" href="foundation.preunivalence.html#2483" class="Bound">B</a>
  <a id="2608" href="foundation.preunivalence.html#2504" class="Function">instance-preunivalence-instance-univalence</a> <a id="2651" class="Symbol">=</a> <a id="2653" href="foundation-core.equivalences.html#19799" class="Function">is-emb-is-equiv</a>

<a id="preunivalence-axiom-univalence-axiom"></a><a id="2670" href="foundation.preunivalence.html#2670" class="Function">preunivalence-axiom-univalence-axiom</a> <a id="2707" class="Symbol">:</a> <a id="2709" href="foundation-core.univalence.html#1405" class="Function">univalence-axiom</a> <a id="2726" class="Symbol">→</a> <a id="2728" href="foundation.preunivalence.html#1212" class="Function">preunivalence-axiom</a>
<a id="2748" href="foundation.preunivalence.html#2670" class="Function">preunivalence-axiom-univalence-axiom</a> <a id="2785" href="foundation.preunivalence.html#2785" class="Bound">UA</a> <a id="2788" href="foundation.preunivalence.html#2788" class="Bound">X</a> <a id="2790" href="foundation.preunivalence.html#2790" class="Bound">Y</a> <a id="2792" class="Symbol">=</a>
  <a id="2796" href="foundation.preunivalence.html#2504" class="Function">instance-preunivalence-instance-univalence</a> <a id="2839" href="foundation.preunivalence.html#2788" class="Bound">X</a> <a id="2841" href="foundation.preunivalence.html#2790" class="Bound">Y</a> <a id="2843" class="Symbol">(</a><a id="2844" href="foundation.preunivalence.html#2785" class="Bound">UA</a> <a id="2847" href="foundation.preunivalence.html#2788" class="Bound">X</a> <a id="2849" href="foundation.preunivalence.html#2790" class="Bound">Y</a><a id="2850" class="Symbol">)</a>
</pre>
### Preunivalence holds in univalent foundations

<pre class="Agda"><a id="preunivalence"></a><a id="2915" href="foundation.preunivalence.html#2915" class="Function">preunivalence</a> <a id="2929" class="Symbol">:</a> <a id="2931" href="foundation.preunivalence.html#1212" class="Function">preunivalence-axiom</a>
<a id="2951" href="foundation.preunivalence.html#2915" class="Function">preunivalence</a> <a id="2965" class="Symbol">=</a> <a id="2967" href="foundation.preunivalence.html#2670" class="Function">preunivalence-axiom-univalence-axiom</a> <a id="3004" href="foundation.univalence.html#1273" class="Postulate">univalence</a>
</pre>
## See also

- Preunivalence is sufficient to prove that `Id : A → (A → 𝒰)` is an embedding.
  This fact is proven in
  [`foundation.universal-property-identity-types`](foundation.universal-property-identity-types.md)
- [Preunivalent categories](category-theory.preunivalent-categories.md)
