# Dependent homotopies

<pre class="Agda"><a id="33" class="Keyword">module</a> <a id="40" href="foundation.dependent-homotopies.html" class="Module">foundation.dependent-homotopies</a> <a id="72" class="Keyword">where</a>
</pre>
<details><summary>Imports</summary>

<pre class="Agda"><a id="128" class="Keyword">open</a> <a id="133" class="Keyword">import</a> <a id="140" href="foundation.universe-levels.html" class="Module">foundation.universe-levels</a>

<a id="168" class="Keyword">open</a> <a id="173" class="Keyword">import</a> <a id="180" href="foundation-core.dependent-identifications.html" class="Module">foundation-core.dependent-identifications</a>
<a id="222" class="Keyword">open</a> <a id="227" class="Keyword">import</a> <a id="234" href="foundation-core.homotopies.html" class="Module">foundation-core.homotopies</a>
</pre>
</details>

## Idea

Consider a [homotopy](foundation-core.homotopies.md) `H : f ~ g` between two
functions `f g : (x : A) → B x`. Furthermore, consider a type family
`C : (x : A) → B x → 𝒰` and two functions

```text
  f' : (x : A) → C x (f x)
  g' : (x : A) → C x (g x)
```

A **dependent homotopy** from `f'` to `g'` over `H` is a family of
[dependent identifications](foundation-core.dependent-identifications.md) from
`f' x` to `g' x` over `H x`.

## Definitions

### Dependent homotopies

<pre class="Agda"><a id="769" class="Keyword">module</a> <a id="776" href="foundation.dependent-homotopies.html#776" class="Module">_</a>
  <a id="780" class="Symbol">{</a><a id="781" href="foundation.dependent-homotopies.html#781" class="Bound">l1</a> <a id="784" href="foundation.dependent-homotopies.html#784" class="Bound">l2</a> <a id="787" href="foundation.dependent-homotopies.html#787" class="Bound">l3</a> <a id="790" class="Symbol">:</a> <a id="792" href="Agda.Primitive.html#742" class="Postulate">Level</a><a id="797" class="Symbol">}</a> <a id="799" class="Symbol">{</a><a id="800" href="foundation.dependent-homotopies.html#800" class="Bound">A</a> <a id="802" class="Symbol">:</a> <a id="804" href="Agda.Primitive.html#388" class="Primitive">UU</a> <a id="807" href="foundation.dependent-homotopies.html#781" class="Bound">l1</a><a id="809" class="Symbol">}</a> <a id="811" class="Symbol">{</a><a id="812" href="foundation.dependent-homotopies.html#812" class="Bound">B</a> <a id="814" class="Symbol">:</a> <a id="816" href="foundation.dependent-homotopies.html#800" class="Bound">A</a> <a id="818" class="Symbol">→</a> <a id="820" href="Agda.Primitive.html#388" class="Primitive">UU</a> <a id="823" href="foundation.dependent-homotopies.html#784" class="Bound">l2</a><a id="825" class="Symbol">}</a> <a id="827" class="Symbol">(</a><a id="828" href="foundation.dependent-homotopies.html#828" class="Bound">C</a> <a id="830" class="Symbol">:</a> <a id="832" class="Symbol">(</a><a id="833" href="foundation.dependent-homotopies.html#833" class="Bound">x</a> <a id="835" class="Symbol">:</a> <a id="837" href="foundation.dependent-homotopies.html#800" class="Bound">A</a><a id="838" class="Symbol">)</a> <a id="840" class="Symbol">→</a> <a id="842" href="foundation.dependent-homotopies.html#812" class="Bound">B</a> <a id="844" href="foundation.dependent-homotopies.html#833" class="Bound">x</a> <a id="846" class="Symbol">→</a> <a id="848" href="Agda.Primitive.html#388" class="Primitive">UU</a> <a id="851" href="foundation.dependent-homotopies.html#787" class="Bound">l3</a><a id="853" class="Symbol">)</a>
  <a id="857" class="Symbol">{</a><a id="858" href="foundation.dependent-homotopies.html#858" class="Bound">f</a> <a id="860" href="foundation.dependent-homotopies.html#860" class="Bound">g</a> <a id="862" class="Symbol">:</a> <a id="864" class="Symbol">(</a><a id="865" href="foundation.dependent-homotopies.html#865" class="Bound">x</a> <a id="867" class="Symbol">:</a> <a id="869" href="foundation.dependent-homotopies.html#800" class="Bound">A</a><a id="870" class="Symbol">)</a> <a id="872" class="Symbol">→</a> <a id="874" href="foundation.dependent-homotopies.html#812" class="Bound">B</a> <a id="876" href="foundation.dependent-homotopies.html#865" class="Bound">x</a><a id="877" class="Symbol">}</a> <a id="879" class="Symbol">(</a><a id="880" href="foundation.dependent-homotopies.html#880" class="Bound">H</a> <a id="882" class="Symbol">:</a> <a id="884" href="foundation.dependent-homotopies.html#858" class="Bound">f</a> <a id="886" href="foundation-core.homotopies.html#2717" class="Function Operator">~</a> <a id="888" href="foundation.dependent-homotopies.html#860" class="Bound">g</a><a id="889" class="Symbol">)</a>
  <a id="893" class="Keyword">where</a>

  <a id="902" href="foundation.dependent-homotopies.html#902" class="Function">dependent-homotopy</a> <a id="921" class="Symbol">:</a>
    <a id="927" class="Symbol">((</a><a id="929" href="foundation.dependent-homotopies.html#929" class="Bound">x</a> <a id="931" class="Symbol">:</a> <a id="933" href="foundation.dependent-homotopies.html#800" class="Bound">A</a><a id="934" class="Symbol">)</a> <a id="936" class="Symbol">→</a> <a id="938" href="foundation.dependent-homotopies.html#828" class="Bound">C</a> <a id="940" href="foundation.dependent-homotopies.html#929" class="Bound">x</a> <a id="942" class="Symbol">(</a><a id="943" href="foundation.dependent-homotopies.html#858" class="Bound">f</a> <a id="945" href="foundation.dependent-homotopies.html#929" class="Bound">x</a><a id="946" class="Symbol">))</a> <a id="949" class="Symbol">→</a> <a id="951" class="Symbol">((</a><a id="953" href="foundation.dependent-homotopies.html#953" class="Bound">x</a> <a id="955" class="Symbol">:</a> <a id="957" href="foundation.dependent-homotopies.html#800" class="Bound">A</a><a id="958" class="Symbol">)</a> <a id="960" class="Symbol">→</a> <a id="962" href="foundation.dependent-homotopies.html#828" class="Bound">C</a> <a id="964" href="foundation.dependent-homotopies.html#953" class="Bound">x</a> <a id="966" class="Symbol">(</a><a id="967" href="foundation.dependent-homotopies.html#860" class="Bound">g</a> <a id="969" href="foundation.dependent-homotopies.html#953" class="Bound">x</a><a id="970" class="Symbol">))</a> <a id="973" class="Symbol">→</a> <a id="975" href="Agda.Primitive.html#388" class="Primitive">UU</a> <a id="978" class="Symbol">(</a><a id="979" href="foundation.dependent-homotopies.html#781" class="Bound">l1</a> <a id="982" href="Agda.Primitive.html#961" class="Primitive Operator">⊔</a> <a id="984" href="foundation.dependent-homotopies.html#787" class="Bound">l3</a><a id="986" class="Symbol">)</a>
  <a id="990" href="foundation.dependent-homotopies.html#902" class="Function">dependent-homotopy</a> <a id="1009" href="foundation.dependent-homotopies.html#1009" class="Bound">f&#39;</a> <a id="1012" href="foundation.dependent-homotopies.html#1012" class="Bound">g&#39;</a> <a id="1015" class="Symbol">=</a>
    <a id="1021" class="Symbol">(</a><a id="1022" href="foundation.dependent-homotopies.html#1022" class="Bound">x</a> <a id="1024" class="Symbol">:</a> <a id="1026" href="foundation.dependent-homotopies.html#800" class="Bound">A</a><a id="1027" class="Symbol">)</a> <a id="1029" class="Symbol">→</a> <a id="1031" href="foundation-core.dependent-identifications.html#964" class="Function">dependent-identification</a> <a id="1056" class="Symbol">(</a><a id="1057" href="foundation.dependent-homotopies.html#828" class="Bound">C</a> <a id="1059" href="foundation.dependent-homotopies.html#1022" class="Bound">x</a><a id="1060" class="Symbol">)</a> <a id="1062" class="Symbol">(</a><a id="1063" href="foundation.dependent-homotopies.html#880" class="Bound">H</a> <a id="1065" href="foundation.dependent-homotopies.html#1022" class="Bound">x</a><a id="1066" class="Symbol">)</a> <a id="1068" class="Symbol">(</a><a id="1069" href="foundation.dependent-homotopies.html#1009" class="Bound">f&#39;</a> <a id="1072" href="foundation.dependent-homotopies.html#1022" class="Bound">x</a><a id="1073" class="Symbol">)</a> <a id="1075" class="Symbol">(</a><a id="1076" href="foundation.dependent-homotopies.html#1012" class="Bound">g&#39;</a> <a id="1079" href="foundation.dependent-homotopies.html#1022" class="Bound">x</a><a id="1080" class="Symbol">)</a>
</pre>
### The reflexive dependent homotopy

<pre class="Agda"><a id="1133" class="Keyword">module</a> <a id="1140" href="foundation.dependent-homotopies.html#1140" class="Module">_</a>
  <a id="1144" class="Symbol">{</a><a id="1145" href="foundation.dependent-homotopies.html#1145" class="Bound">l1</a> <a id="1148" href="foundation.dependent-homotopies.html#1148" class="Bound">l2</a> <a id="1151" href="foundation.dependent-homotopies.html#1151" class="Bound">l3</a> <a id="1154" class="Symbol">:</a> <a id="1156" href="Agda.Primitive.html#742" class="Postulate">Level</a><a id="1161" class="Symbol">}</a> <a id="1163" class="Symbol">{</a><a id="1164" href="foundation.dependent-homotopies.html#1164" class="Bound">A</a> <a id="1166" class="Symbol">:</a> <a id="1168" href="Agda.Primitive.html#388" class="Primitive">UU</a> <a id="1171" href="foundation.dependent-homotopies.html#1145" class="Bound">l1</a><a id="1173" class="Symbol">}</a> <a id="1175" class="Symbol">{</a><a id="1176" href="foundation.dependent-homotopies.html#1176" class="Bound">B</a> <a id="1178" class="Symbol">:</a> <a id="1180" href="foundation.dependent-homotopies.html#1164" class="Bound">A</a> <a id="1182" class="Symbol">→</a> <a id="1184" href="Agda.Primitive.html#388" class="Primitive">UU</a> <a id="1187" href="foundation.dependent-homotopies.html#1148" class="Bound">l2</a><a id="1189" class="Symbol">}</a> <a id="1191" class="Symbol">(</a><a id="1192" href="foundation.dependent-homotopies.html#1192" class="Bound">C</a> <a id="1194" class="Symbol">:</a> <a id="1196" class="Symbol">(</a><a id="1197" href="foundation.dependent-homotopies.html#1197" class="Bound">x</a> <a id="1199" class="Symbol">:</a> <a id="1201" href="foundation.dependent-homotopies.html#1164" class="Bound">A</a><a id="1202" class="Symbol">)</a> <a id="1204" class="Symbol">→</a> <a id="1206" href="foundation.dependent-homotopies.html#1176" class="Bound">B</a> <a id="1208" href="foundation.dependent-homotopies.html#1197" class="Bound">x</a> <a id="1210" class="Symbol">→</a> <a id="1212" href="Agda.Primitive.html#388" class="Primitive">UU</a> <a id="1215" href="foundation.dependent-homotopies.html#1151" class="Bound">l3</a><a id="1217" class="Symbol">)</a>
  <a id="1221" class="Symbol">{</a><a id="1222" href="foundation.dependent-homotopies.html#1222" class="Bound">f</a> <a id="1224" class="Symbol">:</a> <a id="1226" class="Symbol">(</a><a id="1227" href="foundation.dependent-homotopies.html#1227" class="Bound">x</a> <a id="1229" class="Symbol">:</a> <a id="1231" href="foundation.dependent-homotopies.html#1164" class="Bound">A</a><a id="1232" class="Symbol">)</a> <a id="1234" class="Symbol">→</a> <a id="1236" href="foundation.dependent-homotopies.html#1176" class="Bound">B</a> <a id="1238" href="foundation.dependent-homotopies.html#1227" class="Bound">x</a><a id="1239" class="Symbol">}</a>
  <a id="1243" class="Keyword">where</a>

  <a id="1252" href="foundation.dependent-homotopies.html#1252" class="Function">refl-dependent-homotopy</a> <a id="1276" class="Symbol">:</a>
    <a id="1282" class="Symbol">{</a><a id="1283" href="foundation.dependent-homotopies.html#1283" class="Bound">f&#39;</a> <a id="1286" class="Symbol">:</a> <a id="1288" class="Symbol">(</a><a id="1289" href="foundation.dependent-homotopies.html#1289" class="Bound">x</a> <a id="1291" class="Symbol">:</a> <a id="1293" href="foundation.dependent-homotopies.html#1164" class="Bound">A</a><a id="1294" class="Symbol">)</a> <a id="1296" class="Symbol">→</a> <a id="1298" href="foundation.dependent-homotopies.html#1192" class="Bound">C</a> <a id="1300" href="foundation.dependent-homotopies.html#1289" class="Bound">x</a> <a id="1302" class="Symbol">(</a><a id="1303" href="foundation.dependent-homotopies.html#1222" class="Bound">f</a> <a id="1305" href="foundation.dependent-homotopies.html#1289" class="Bound">x</a><a id="1306" class="Symbol">)}</a> <a id="1309" class="Symbol">→</a> <a id="1311" href="foundation.dependent-homotopies.html#902" class="Function">dependent-homotopy</a> <a id="1330" href="foundation.dependent-homotopies.html#1192" class="Bound">C</a> <a id="1332" href="foundation-core.homotopies.html#2906" class="Function">refl-htpy</a> <a id="1342" href="foundation.dependent-homotopies.html#1283" class="Bound">f&#39;</a> <a id="1345" href="foundation.dependent-homotopies.html#1283" class="Bound">f&#39;</a>
  <a id="1350" href="foundation.dependent-homotopies.html#1252" class="Function">refl-dependent-homotopy</a> <a id="1374" class="Symbol">=</a> <a id="1376" href="foundation-core.homotopies.html#2906" class="Function">refl-htpy</a>
</pre>
### Iterated dependent homotopies

<pre class="Agda"><a id="1434" class="Keyword">module</a> <a id="1441" href="foundation.dependent-homotopies.html#1441" class="Module">_</a>
  <a id="1445" class="Symbol">{</a><a id="1446" href="foundation.dependent-homotopies.html#1446" class="Bound">l1</a> <a id="1449" href="foundation.dependent-homotopies.html#1449" class="Bound">l2</a> <a id="1452" href="foundation.dependent-homotopies.html#1452" class="Bound">l3</a> <a id="1455" class="Symbol">:</a> <a id="1457" href="Agda.Primitive.html#742" class="Postulate">Level</a><a id="1462" class="Symbol">}</a> <a id="1464" class="Symbol">{</a><a id="1465" href="foundation.dependent-homotopies.html#1465" class="Bound">A</a> <a id="1467" class="Symbol">:</a> <a id="1469" href="Agda.Primitive.html#388" class="Primitive">UU</a> <a id="1472" href="foundation.dependent-homotopies.html#1446" class="Bound">l1</a><a id="1474" class="Symbol">}</a> <a id="1476" class="Symbol">{</a><a id="1477" href="foundation.dependent-homotopies.html#1477" class="Bound">B</a> <a id="1479" class="Symbol">:</a> <a id="1481" href="foundation.dependent-homotopies.html#1465" class="Bound">A</a> <a id="1483" class="Symbol">→</a> <a id="1485" href="Agda.Primitive.html#388" class="Primitive">UU</a> <a id="1488" href="foundation.dependent-homotopies.html#1449" class="Bound">l2</a><a id="1490" class="Symbol">}</a> <a id="1492" class="Symbol">(</a><a id="1493" href="foundation.dependent-homotopies.html#1493" class="Bound">C</a> <a id="1495" class="Symbol">:</a> <a id="1497" class="Symbol">(</a><a id="1498" href="foundation.dependent-homotopies.html#1498" class="Bound">x</a> <a id="1500" class="Symbol">:</a> <a id="1502" href="foundation.dependent-homotopies.html#1465" class="Bound">A</a><a id="1503" class="Symbol">)</a> <a id="1505" class="Symbol">→</a> <a id="1507" href="foundation.dependent-homotopies.html#1477" class="Bound">B</a> <a id="1509" href="foundation.dependent-homotopies.html#1498" class="Bound">x</a> <a id="1511" class="Symbol">→</a> <a id="1513" href="Agda.Primitive.html#388" class="Primitive">UU</a> <a id="1516" href="foundation.dependent-homotopies.html#1452" class="Bound">l3</a><a id="1518" class="Symbol">)</a>
  <a id="1522" class="Symbol">{</a><a id="1523" href="foundation.dependent-homotopies.html#1523" class="Bound">f</a> <a id="1525" href="foundation.dependent-homotopies.html#1525" class="Bound">g</a> <a id="1527" class="Symbol">:</a> <a id="1529" class="Symbol">(</a><a id="1530" href="foundation.dependent-homotopies.html#1530" class="Bound">x</a> <a id="1532" class="Symbol">:</a> <a id="1534" href="foundation.dependent-homotopies.html#1465" class="Bound">A</a><a id="1535" class="Symbol">)</a> <a id="1537" class="Symbol">→</a> <a id="1539" href="foundation.dependent-homotopies.html#1477" class="Bound">B</a> <a id="1541" href="foundation.dependent-homotopies.html#1530" class="Bound">x</a><a id="1542" class="Symbol">}</a> <a id="1544" class="Symbol">{</a><a id="1545" href="foundation.dependent-homotopies.html#1545" class="Bound">H</a> <a id="1547" href="foundation.dependent-homotopies.html#1547" class="Bound">K</a> <a id="1549" class="Symbol">:</a> <a id="1551" href="foundation.dependent-homotopies.html#1523" class="Bound">f</a> <a id="1553" href="foundation-core.homotopies.html#2717" class="Function Operator">~</a> <a id="1555" href="foundation.dependent-homotopies.html#1525" class="Bound">g</a><a id="1556" class="Symbol">}</a> <a id="1558" class="Symbol">(</a><a id="1559" href="foundation.dependent-homotopies.html#1559" class="Bound">L</a> <a id="1561" class="Symbol">:</a> <a id="1563" href="foundation.dependent-homotopies.html#1545" class="Bound">H</a> <a id="1565" href="foundation-core.homotopies.html#2717" class="Function Operator">~</a> <a id="1567" href="foundation.dependent-homotopies.html#1547" class="Bound">K</a><a id="1568" class="Symbol">)</a>
  <a id="1572" class="Keyword">where</a>

  <a id="1581" href="foundation.dependent-homotopies.html#1581" class="Function">dependent-homotopy²</a> <a id="1601" class="Symbol">:</a>
    <a id="1607" class="Symbol">{</a><a id="1608" href="foundation.dependent-homotopies.html#1608" class="Bound">f&#39;</a> <a id="1611" class="Symbol">:</a> <a id="1613" class="Symbol">(</a><a id="1614" href="foundation.dependent-homotopies.html#1614" class="Bound">x</a> <a id="1616" class="Symbol">:</a> <a id="1618" href="foundation.dependent-homotopies.html#1465" class="Bound">A</a><a id="1619" class="Symbol">)</a> <a id="1621" class="Symbol">→</a> <a id="1623" href="foundation.dependent-homotopies.html#1493" class="Bound">C</a> <a id="1625" href="foundation.dependent-homotopies.html#1614" class="Bound">x</a> <a id="1627" class="Symbol">(</a><a id="1628" href="foundation.dependent-homotopies.html#1523" class="Bound">f</a> <a id="1630" href="foundation.dependent-homotopies.html#1614" class="Bound">x</a><a id="1631" class="Symbol">)}</a> <a id="1634" class="Symbol">{</a><a id="1635" href="foundation.dependent-homotopies.html#1635" class="Bound">g&#39;</a> <a id="1638" class="Symbol">:</a> <a id="1640" class="Symbol">(</a><a id="1641" href="foundation.dependent-homotopies.html#1641" class="Bound">x</a> <a id="1643" class="Symbol">:</a> <a id="1645" href="foundation.dependent-homotopies.html#1465" class="Bound">A</a><a id="1646" class="Symbol">)</a> <a id="1648" class="Symbol">→</a> <a id="1650" href="foundation.dependent-homotopies.html#1493" class="Bound">C</a> <a id="1652" href="foundation.dependent-homotopies.html#1641" class="Bound">x</a> <a id="1654" class="Symbol">(</a><a id="1655" href="foundation.dependent-homotopies.html#1525" class="Bound">g</a> <a id="1657" href="foundation.dependent-homotopies.html#1641" class="Bound">x</a><a id="1658" class="Symbol">)}</a> <a id="1661" class="Symbol">→</a>
    <a id="1667" href="foundation.dependent-homotopies.html#902" class="Function">dependent-homotopy</a> <a id="1686" href="foundation.dependent-homotopies.html#1493" class="Bound">C</a> <a id="1688" href="foundation.dependent-homotopies.html#1545" class="Bound">H</a> <a id="1690" href="foundation.dependent-homotopies.html#1608" class="Bound">f&#39;</a> <a id="1693" href="foundation.dependent-homotopies.html#1635" class="Bound">g&#39;</a> <a id="1696" class="Symbol">→</a>
    <a id="1702" href="foundation.dependent-homotopies.html#902" class="Function">dependent-homotopy</a> <a id="1721" href="foundation.dependent-homotopies.html#1493" class="Bound">C</a> <a id="1723" href="foundation.dependent-homotopies.html#1547" class="Bound">K</a> <a id="1725" href="foundation.dependent-homotopies.html#1608" class="Bound">f&#39;</a> <a id="1728" href="foundation.dependent-homotopies.html#1635" class="Bound">g&#39;</a> <a id="1731" class="Symbol">→</a> <a id="1733" href="Agda.Primitive.html#388" class="Primitive">UU</a> <a id="1736" class="Symbol">(</a><a id="1737" href="foundation.dependent-homotopies.html#1446" class="Bound">l1</a> <a id="1740" href="Agda.Primitive.html#961" class="Primitive Operator">⊔</a> <a id="1742" href="foundation.dependent-homotopies.html#1452" class="Bound">l3</a><a id="1744" class="Symbol">)</a>
  <a id="1748" href="foundation.dependent-homotopies.html#1581" class="Function">dependent-homotopy²</a> <a id="1768" class="Symbol">{</a><a id="1769" href="foundation.dependent-homotopies.html#1769" class="Bound">f&#39;</a><a id="1771" class="Symbol">}</a> <a id="1773" class="Symbol">{</a><a id="1774" href="foundation.dependent-homotopies.html#1774" class="Bound">g&#39;</a><a id="1776" class="Symbol">}</a> <a id="1778" href="foundation.dependent-homotopies.html#1778" class="Bound">H&#39;</a> <a id="1781" href="foundation.dependent-homotopies.html#1781" class="Bound">K&#39;</a> <a id="1784" class="Symbol">=</a>
    <a id="1790" class="Symbol">(</a><a id="1791" href="foundation.dependent-homotopies.html#1791" class="Bound">x</a> <a id="1793" class="Symbol">:</a> <a id="1795" href="foundation.dependent-homotopies.html#1465" class="Bound">A</a><a id="1796" class="Symbol">)</a> <a id="1798" class="Symbol">→</a> <a id="1800" href="foundation-core.dependent-identifications.html#1429" class="Function">dependent-identification²</a> <a id="1826" class="Symbol">(</a><a id="1827" href="foundation.dependent-homotopies.html#1493" class="Bound">C</a> <a id="1829" href="foundation.dependent-homotopies.html#1791" class="Bound">x</a><a id="1830" class="Symbol">)</a> <a id="1832" class="Symbol">(</a><a id="1833" href="foundation.dependent-homotopies.html#1559" class="Bound">L</a> <a id="1835" href="foundation.dependent-homotopies.html#1791" class="Bound">x</a><a id="1836" class="Symbol">)</a> <a id="1838" class="Symbol">(</a><a id="1839" href="foundation.dependent-homotopies.html#1778" class="Bound">H&#39;</a> <a id="1842" href="foundation.dependent-homotopies.html#1791" class="Bound">x</a><a id="1843" class="Symbol">)</a> <a id="1845" class="Symbol">(</a><a id="1846" href="foundation.dependent-homotopies.html#1781" class="Bound">K&#39;</a> <a id="1849" href="foundation.dependent-homotopies.html#1791" class="Bound">x</a><a id="1850" class="Symbol">)</a>
</pre>