# Hilbert's `ε`-operators

<pre class="Agda"><a id="36" class="Keyword">module</a> <a id="43" href="foundation.hilberts-epsilon-operators.html" class="Module">foundation.hilberts-epsilon-operators</a> <a id="81" class="Keyword">where</a>
</pre>
<details><summary>Imports</summary>

<pre class="Agda"><a id="137" class="Keyword">open</a> <a id="142" class="Keyword">import</a> <a id="149" href="foundation.functoriality-propositional-truncation.html" class="Module">foundation.functoriality-propositional-truncation</a>
<a id="199" class="Keyword">open</a> <a id="204" class="Keyword">import</a> <a id="211" href="foundation.propositional-truncations.html" class="Module">foundation.propositional-truncations</a>
<a id="248" class="Keyword">open</a> <a id="253" class="Keyword">import</a> <a id="260" href="foundation.universe-levels.html" class="Module">foundation.universe-levels</a>

<a id="288" class="Keyword">open</a> <a id="293" class="Keyword">import</a> <a id="300" href="foundation-core.equivalences.html" class="Module">foundation-core.equivalences</a>
<a id="329" class="Keyword">open</a> <a id="334" class="Keyword">import</a> <a id="341" href="foundation-core.function-types.html" class="Module">foundation-core.function-types</a>
</pre>
</details>

## Idea

Hilbert's $ε$-operator at a type `A` is a map `type-trunc-Prop A → A`. Contrary
to Hilbert, we will not assume that such an operator exists for each type `A`.

## Definition

<pre class="Agda"><a id="ε-operator-Hilbert"></a><a id="581" href="foundation.hilberts-epsilon-operators.html#581" class="Function">ε-operator-Hilbert</a> <a id="600" class="Symbol">:</a> <a id="602" class="Symbol">{</a><a id="603" href="foundation.hilberts-epsilon-operators.html#603" class="Bound">l</a> <a id="605" class="Symbol">:</a> <a id="607" href="Agda.Primitive.html#742" class="Postulate">Level</a><a id="612" class="Symbol">}</a> <a id="614" class="Symbol">→</a> <a id="616" href="Agda.Primitive.html#388" class="Primitive">UU</a> <a id="619" href="foundation.hilberts-epsilon-operators.html#603" class="Bound">l</a> <a id="621" class="Symbol">→</a> <a id="623" href="Agda.Primitive.html#388" class="Primitive">UU</a> <a id="626" href="foundation.hilberts-epsilon-operators.html#603" class="Bound">l</a>
<a id="628" href="foundation.hilberts-epsilon-operators.html#581" class="Function">ε-operator-Hilbert</a> <a id="647" href="foundation.hilberts-epsilon-operators.html#647" class="Bound">A</a> <a id="649" class="Symbol">=</a> <a id="651" href="foundation.propositional-truncations.html#1383" class="Function">type-trunc-Prop</a> <a id="667" href="foundation.hilberts-epsilon-operators.html#647" class="Bound">A</a> <a id="669" class="Symbol">→</a> <a id="671" href="foundation.hilberts-epsilon-operators.html#647" class="Bound">A</a>
</pre>
## Properties

### The existence of Hilbert's `ε`-operators is invariant under equivalences

<pre class="Agda"><a id="ε-operator-equiv"></a><a id="779" href="foundation.hilberts-epsilon-operators.html#779" class="Function">ε-operator-equiv</a> <a id="796" class="Symbol">:</a>
  <a id="800" class="Symbol">{</a><a id="801" href="foundation.hilberts-epsilon-operators.html#801" class="Bound">l1</a> <a id="804" href="foundation.hilberts-epsilon-operators.html#804" class="Bound">l2</a> <a id="807" class="Symbol">:</a> <a id="809" href="Agda.Primitive.html#742" class="Postulate">Level</a><a id="814" class="Symbol">}</a> <a id="816" class="Symbol">{</a><a id="817" href="foundation.hilberts-epsilon-operators.html#817" class="Bound">X</a> <a id="819" class="Symbol">:</a> <a id="821" href="Agda.Primitive.html#388" class="Primitive">UU</a> <a id="824" href="foundation.hilberts-epsilon-operators.html#801" class="Bound">l1</a><a id="826" class="Symbol">}</a> <a id="828" class="Symbol">{</a><a id="829" href="foundation.hilberts-epsilon-operators.html#829" class="Bound">Y</a> <a id="831" class="Symbol">:</a> <a id="833" href="Agda.Primitive.html#388" class="Primitive">UU</a> <a id="836" href="foundation.hilberts-epsilon-operators.html#804" class="Bound">l2</a><a id="838" class="Symbol">}</a> <a id="840" class="Symbol">(</a><a id="841" href="foundation.hilberts-epsilon-operators.html#841" class="Bound">e</a> <a id="843" class="Symbol">:</a> <a id="845" href="foundation.hilberts-epsilon-operators.html#817" class="Bound">X</a> <a id="847" href="foundation-core.equivalences.html#2669" class="Function Operator">≃</a> <a id="849" href="foundation.hilberts-epsilon-operators.html#829" class="Bound">Y</a><a id="850" class="Symbol">)</a> <a id="852" class="Symbol">→</a>
  <a id="856" href="foundation.hilberts-epsilon-operators.html#581" class="Function">ε-operator-Hilbert</a> <a id="875" href="foundation.hilberts-epsilon-operators.html#817" class="Bound">X</a> <a id="877" class="Symbol">→</a> <a id="879" href="foundation.hilberts-epsilon-operators.html#581" class="Function">ε-operator-Hilbert</a> <a id="898" href="foundation.hilberts-epsilon-operators.html#829" class="Bound">Y</a>
<a id="900" href="foundation.hilberts-epsilon-operators.html#779" class="Function">ε-operator-equiv</a> <a id="917" href="foundation.hilberts-epsilon-operators.html#917" class="Bound">e</a> <a id="919" href="foundation.hilberts-epsilon-operators.html#919" class="Bound">f</a> <a id="921" class="Symbol">=</a>
  <a id="925" class="Symbol">(</a><a id="926" href="foundation-core.equivalences.html#2869" class="Function">map-equiv</a> <a id="936" href="foundation.hilberts-epsilon-operators.html#917" class="Bound">e</a> <a id="938" href="foundation-core.function-types.html#455" class="Function Operator">∘</a> <a id="940" href="foundation.hilberts-epsilon-operators.html#919" class="Bound">f</a><a id="941" class="Symbol">)</a> <a id="943" href="foundation-core.function-types.html#455" class="Function Operator">∘</a> <a id="945" class="Symbol">(</a><a id="946" href="foundation.functoriality-propositional-truncation.html#1209" class="Function">map-trunc-Prop</a> <a id="961" class="Symbol">(</a><a id="962" href="foundation-core.equivalences.html#7679" class="Function">map-inv-equiv</a> <a id="976" href="foundation.hilberts-epsilon-operators.html#917" class="Bound">e</a><a id="977" class="Symbol">))</a>

<a id="ε-operator-equiv&#39;"></a><a id="981" href="foundation.hilberts-epsilon-operators.html#981" class="Function">ε-operator-equiv&#39;</a> <a id="999" class="Symbol">:</a>
  <a id="1003" class="Symbol">{</a><a id="1004" href="foundation.hilberts-epsilon-operators.html#1004" class="Bound">l1</a> <a id="1007" href="foundation.hilberts-epsilon-operators.html#1007" class="Bound">l2</a> <a id="1010" class="Symbol">:</a> <a id="1012" href="Agda.Primitive.html#742" class="Postulate">Level</a><a id="1017" class="Symbol">}</a> <a id="1019" class="Symbol">{</a><a id="1020" href="foundation.hilberts-epsilon-operators.html#1020" class="Bound">X</a> <a id="1022" class="Symbol">:</a> <a id="1024" href="Agda.Primitive.html#388" class="Primitive">UU</a> <a id="1027" href="foundation.hilberts-epsilon-operators.html#1004" class="Bound">l1</a><a id="1029" class="Symbol">}</a> <a id="1031" class="Symbol">{</a><a id="1032" href="foundation.hilberts-epsilon-operators.html#1032" class="Bound">Y</a> <a id="1034" class="Symbol">:</a> <a id="1036" href="Agda.Primitive.html#388" class="Primitive">UU</a> <a id="1039" href="foundation.hilberts-epsilon-operators.html#1007" class="Bound">l2</a><a id="1041" class="Symbol">}</a> <a id="1043" class="Symbol">(</a><a id="1044" href="foundation.hilberts-epsilon-operators.html#1044" class="Bound">e</a> <a id="1046" class="Symbol">:</a> <a id="1048" href="foundation.hilberts-epsilon-operators.html#1020" class="Bound">X</a> <a id="1050" href="foundation-core.equivalences.html#2669" class="Function Operator">≃</a> <a id="1052" href="foundation.hilberts-epsilon-operators.html#1032" class="Bound">Y</a><a id="1053" class="Symbol">)</a> <a id="1055" class="Symbol">→</a>
  <a id="1059" href="foundation.hilberts-epsilon-operators.html#581" class="Function">ε-operator-Hilbert</a> <a id="1078" href="foundation.hilberts-epsilon-operators.html#1032" class="Bound">Y</a> <a id="1080" class="Symbol">→</a> <a id="1082" href="foundation.hilberts-epsilon-operators.html#581" class="Function">ε-operator-Hilbert</a> <a id="1101" href="foundation.hilberts-epsilon-operators.html#1020" class="Bound">X</a>
<a id="1103" href="foundation.hilberts-epsilon-operators.html#981" class="Function">ε-operator-equiv&#39;</a> <a id="1121" href="foundation.hilberts-epsilon-operators.html#1121" class="Bound">e</a> <a id="1123" href="foundation.hilberts-epsilon-operators.html#1123" class="Bound">f</a> <a id="1125" class="Symbol">=</a>
  <a id="1129" class="Symbol">(</a><a id="1130" href="foundation-core.equivalences.html#7679" class="Function">map-inv-equiv</a> <a id="1144" href="foundation.hilberts-epsilon-operators.html#1121" class="Bound">e</a> <a id="1146" href="foundation-core.function-types.html#455" class="Function Operator">∘</a> <a id="1148" href="foundation.hilberts-epsilon-operators.html#1123" class="Bound">f</a><a id="1149" class="Symbol">)</a> <a id="1151" href="foundation-core.function-types.html#455" class="Function Operator">∘</a> <a id="1153" class="Symbol">(</a><a id="1154" href="foundation.functoriality-propositional-truncation.html#1209" class="Function">map-trunc-Prop</a> <a id="1169" class="Symbol">(</a><a id="1170" href="foundation-core.equivalences.html#2869" class="Function">map-equiv</a> <a id="1180" href="foundation.hilberts-epsilon-operators.html#1121" class="Bound">e</a><a id="1181" class="Symbol">))</a>
</pre>